SeparationLogic/DeepEmbeddedInstance/FlatSemantics.v
@@ -2,6 +2,7 @@ Require Import Coq.Logic.Classical_Prop.
 Require Import Coq.Classes.RelationClasses.
 Require Import Coq.Relations.Relation_Definitions.
 Require Import Logic.lib.Coqlib.
+Require Import Logic.lib.Ensembles_ext.
 Require Import Logic.GeneralLogic.Base.
 Require Import Logic.MinimunLogic.Syntax.
 Require Import Logic.PropositionalLogic.Syntax.
@@ -24,12 +25,10 @@ Record frame: Type := {
   underlying_set:> Type;
   Krelation: relation underlying_set; (* <= *)
   Krelation_Preorder: PreOrder Krelation;
-  R: Relation underlying_set := Krelation;
-  kiM: KripkeIntuitionisticModel underlying_set := Krelation_Preorder;
-  J: Join underlying_set;
-  SA: SeparationAlgebra underlying_set;
-  dSA: DownwardsClosedSeparationAlgebra underlying_set;
-  uSA: UpwardsClosedSeparationAlgebra underlying_set
+  Frame_join: Join underlying_set;
+  Frame_SA: SeparationAlgebra underlying_set;
+  Frame_downwards: @DownwardsClosedSeparationAlgebra underlying_set Krelation Frame_join;
+  Frame_upwards: @UpwardsClosedSeparationAlgebra underlying_set Krelation Frame_join
 }.
 
 Infix "<=" := (Krelation _): TheKripkeSemantics.
@@ -44,9 +43,9 @@ Program Definition denotation {Var: Type} (F: frame) (eval_emp: sem F) (eval: Va
   | andp y z => @Semantics.andp F (denotation y) (denotation z)
   | orp y z => Semantics.orp (denotation y) (denotation z)
   | impp y z => @Semantics.impp F (Krelation F) (denotation y) (denotation z)
-  | sepcon y z => @WeakSemantics.sepcon F (J F) (denotation y) (denotation z)
-  | wand y z => @WeakSemantics.wand F (J F) (denotation y) (denotation z)
-  | emp => @WeakSemantics.emp F (Krelation F) (J F)
+  | sepcon y z => @WeakSemantics.sepcon F (Frame_join F) (denotation y) (denotation z)
+  | wand y z => @WeakSemantics.wand F (Frame_join F) (denotation y) (denotation z)
+  | emp => @WeakSemantics.emp F (Krelation F) (Frame_join F)
   | falsep => Semantics.falsep
   | varp p => eval p
   end.
@@ -63,15 +62,15 @@ Next Obligation.
   apply (proj2_sig (denotation _)).
 Defined.
 Next Obligation.
-  apply (@WeakSemantics.sepcon_closed F (Krelation F) (Krelation_Preorder F) (J F) (SA F) (uSA F));
+  apply (@WeakSemantics.sepcon_closed F (Krelation F) (Krelation_Preorder F) (Frame_join F) (Frame_SA F) (Frame_upwards F));
   apply (proj2_sig (denotation _)).
 Defined.
 Next Obligation.
-  apply (@WeakSemantics.wand_closed F (Krelation F) (Krelation_Preorder F) (J F) (SA F) (dSA F));
+  apply (@WeakSemantics.wand_closed F (Krelation F) (Krelation_Preorder F) (Frame_join F) (Frame_SA F) (Frame_downwards F));
   apply (proj2_sig (denotation _)).
 Defined.
 Next Obligation.
-  apply (@WeakSemantics.emp_closed F (Krelation F) (Krelation_Preorder F) (J F) (SA F) (dSA F)).
+  apply (@WeakSemantics.emp_closed F (Krelation F) (Krelation_Preorder F) (Frame_join F) (Frame_SA F) (Frame_downwards F)).
 Defined.
 Next Obligation.
   apply (@Semantics.falsep_closed F (Krelation F)).
@@ -100,39 +99,50 @@ Instance kMD: KripkeModel MD :=
     (fun M => M)
     (fun M m => Build_model M m).
 
-Existing Instances kiM J SA dSA uSA.
-
 Instance SM: Semantics L MD :=
-  Build_Semantics L MD
-   (fun M x => proj1_sig (denotation M (Kemp M) (Kvar M) x) (elm M)).
+  Build_Semantics L MD (fun x M => proj1_sig (denotation M (Kemp M) (Kvar M) x) (elm M)).
+
+Instance R (M: Kmodel): Relation (Kworlds M) :=
+  @Krelation M.
+
+Instance kiM (M: Kmodel): KripkeIntuitionisticModel (Kworlds M) :=
+  @Krelation_Preorder M.
+
+Instance J (M: Kmodel): Join (Kworlds M) :=
+  @Frame_join M.
+
+Instance SA (M: Kmodel): SeparationAlgebra (Kworlds M) :=
+  @Frame_SA M.
+
+Instance uSA (M: Kmodel): UpwardsClosedSeparationAlgebra (Kworlds M) :=
+  @Frame_upwards M.
+
+Instance dSA (M: Kmodel): DownwardsClosedSeparationAlgebra (Kworlds M) :=
+  @Frame_downwards M.
 
 Instance kiSM (M: Kmodel): KripkeIntuitionisticSemantics L MD M SM.
 Proof.
   apply Build_KripkeIntuitionisticSemantics.
   + hnf; simpl; intros.
     eapply (proj2_sig (denotation M (Kemp M) (Kvar M) x)); eauto.
-  + split; auto.
-  + split; auto.
-  + split; auto.
-  + intros; simpl. auto.
+  + intros; apply Same_set_refl.
+  + intros; apply Same_set_refl.
+  + intros; apply Same_set_refl.
+  + intros; apply Same_set_refl.
 Defined.
 
-Instance fsSM (M: Kmodel): FlatSemantics.FlatSemantics L MD M SM.
+Instance fsSM (M: Kmodel): FlatSemantics.SeparatingSemantics L MD M SM.
 Proof.
-  apply FlatSemantics.Build_FlatSemantics.
-  + intros.
-    simpl; reflexivity.
-  + intros.
-    simpl; reflexivity.
+  apply FlatSemantics.Build_SeparatingSemantics.
+  + intros; apply Same_set_refl.
+  + intros; apply Same_set_refl.
 Defined.
 
-(*
-Instance UsSM (M: Kmodel): UnitalSemantics L MD M SM.
+Instance feSM (M: Kmodel): FlatSemantics.EmpSemantics L MD M SM.
 Proof.
   hnf; intros.
-  simpl; reflexivity.
+  intros; apply Same_set_refl.
 Defined.
-*)
 
 Definition Kmodel_Identity: Kmodel -> Prop := fun M =>
   IdentityKripkeIntuitionisticModel (Kworlds M).
@@ -143,27 +153,24 @@ Definition Kmodel_NoBranch: Kmodel -> Prop := fun M =>
 Definition Kmodel_BranchJoin: Kmodel -> Prop := fun M =>
   BranchJoinKripkeIntuitionisticModel (Kworlds M).
 
-(* TODO: the name should be nonpositive *)
-Definition Kmodel_GarbageCollect: Kmodel -> Prop := fun M =>
-  GarbageCollectSeparationAlgebra (Kworlds M).
+Definition Kmodel_Increasing: Kmodel -> Prop := fun M =>
+  IncreasingSeparationAlgebra (Kworlds M).
 
 Definition Kmodel_Unital: Kmodel -> Prop := fun M =>
-  (forall m: Kworlds M, proj1_sig (Kemp M) m <-> proj1_sig sem_emp m) /\
+  (forall m: Kworlds M, proj1_sig (Kemp M) m <-> WeakSemantics.emp m) /\
   UnitalSeparationAlgebra (Kworlds M).
 
 Definition Kmodel_Residual: Kmodel -> Prop := fun M =>
   ResidualSeparationAlgebra (Kworlds M).
 
-
-Require Import Logic.SeparationLogic.SoundCompleteParameter.
+Require Import Logic.SeparationLogic.DeepEmbeddedInstance.Parameter.
 
 Record Kmodel_ParClass (PAR: SA_Parameter) (M: Kmodel): Prop := {
   SA_ID: ID PAR = true -> IdentityKripkeIntuitionisticModel (Kworlds M);
   SA_NB: NB PAR = true -> NoBranchKripkeIntuitionisticModel (Kworlds M);
   SA_BJ: BJ PAR = true -> BranchJoinKripkeIntuitionisticModel (Kworlds M);
-  SA_GC: GC PAR = true -> GarbageCollectSeparationAlgebra (Kworlds M);
+  SA_GC: GC PAR = true -> IncreasingSeparationAlgebra (Kworlds M);
   SA_Uni: Uni PAR = true -> UnitalSeparationAlgebra (Kworlds M)
 }.
 
 End KripkeSemantics.
-End FlatSemanticsModel.
